<?xml version="1.0" encoding="UTF-8"?>

<!--pretext-->
    <!--article xml:id="Sec_2_1"-->
        <section xml:id="Section_2_1">
        <title>Section 2.1</title>
        

<subsection xml:id="Question_2_1_1">
    <title> Problem 1</title>
   
        
     <ol marker="(a)">
        
        <li><!--
            <m>\phantom{empty}</m>
            <p>
               The <m>n^\text{th}</m> triangular number is of the form 
<me>1+2+3+\cdots n.</me>

You can prove this equals <m>\frac{n(n+1)}{2}</m> using induction. 
            </p> -->
        </li>

        <li><!--
            <m>\phantom{empty}</m>
            <p>
              <me>8\cdot \frac{m(m+1)}{2}+1=4m^2+4m+1=(2m+1)^2</me>

            </p>-->
        </li>

        <li><m>\phantom{empty}</m>
            <p>
            <md>
                <mrow>\frac{n(n+1)}{2}+\frac{(n+1)(n+2)}{2}\amp=\frac{(n+1)(2n+2)}{2}</mrow>
                <mrow>\amp=(n+1)^2</mrow>
            </md>
            </p>
        </li>
<!--
        <li> <m>\phantom{empty}</m>
            <p>
                <md>
                    <mrow>9\cdot \frac{m(m+1)}{2}+1\amp=\frac{9m(m+1)+2}{2}</mrow>
                    <mrow>\amp=\frac{9m^2+9m+2}{2}</mrow>       
                    <mrow>\amp=\frac{(3m+1)(3m+2)}{2}</mrow>
                    <mrow>\amp=\frac{k(k+1)}{2}</mrow>
                </md>

where <m>k=3m+1</m>. So, if <m>n=\frac{m(m+1)}{2}</m> is the <m>m^\text{th}</m> triangular number, then <m>9n+1</m> is the <m>(3m+1)^\text{st}</m> triangular number.


            </p>
        </li>
    -->

    </ol>
        
</subsection>        
       
<!--
<subsection xml:id="Question_2_1_2">
    <title> Problem 2</title>
    <p>
        <me>\binom{n+1}{2}=\frac{(n+1)!}{2!\cdot (n-1)!}=\frac{(n+1)(n)}{2}</me>
    </p>
</subsection>

-->

<subsection xml:id="Question_2_1_3">
    <title> Problem 3</title>
    <p>
       The hint follows from question 1(a).

If <m>n</m> is even, let <m>n=2m</m>:

<md>
<mrow>t_1+t_2+\dots+t_n\amp= (t_1+t_2)+(t_3+t_4)+\dots+(t_{n-1}+t_n)</mrow>
<mrow>\amp=2^2+4^2+\dots+(2m)^2</mrow>
<mrow>\amp=2^2(1+2^2+3^2+\dots+m^2)</mrow>
<mrow>\amp=2^2\cdot \left(\frac{m(2m+1)(m+1)}{6}\right)</mrow>
<mrow>\amp=\frac{2m(2m+1)(2m+2)}{6}</mrow>
<mrow>\amp=\frac{n(n+1)(n+2)}{6}</mrow>
</md>

where we have used the result from section 1.1 concerning the sum of the first <m>n</m> squares. 

If <m>n</m> is odd:

<md>
<mrow>t_1+t_2+\dots+t_n\amp= (t_1+t_2)+(t_3+t_4)+\dots+(t_{n-2}+t_{n-1})+t_n</mrow>
<mrow>\amp=\frac{(n-1)(n)(n+1)}{6}+\frac{n(n+1)}{2}</mrow>
<mrow>\amp=\frac{(n-1)(n)(n+1)+3n(n+1)}{6}</mrow>
<mrow>\amp=\frac{(n+1)(n^2-n+3n)}{6}</mrow>
<mrow>\amp=\frac{(n+1)(n)(n+2)}{6}</mrow>
</md>
    </p>
</subsection>

<!--
<subsection xml:id="Question_2_1_6">
    <title> Problem 6</title>
    <p>
       <md>
            <mrow>\frac{4n(n+1)(4n(n+1)+1)}{2}\amp=\frac{(4n^2+4n)(4n^2+4n+1)}{2}</mrow>
            <mrow>\amp=\frac{4n(n+1)(2n+1)^2}{2}</mrow>
            <mrow>\amp=\frac{n(n+1)}{2}\cdot \left(2(2n+1)\right)^2</mrow>
       </md>

The first triangular number that is also a square is 1. Use this to find another: <me>t_{4(1)((1)+1)}=t_8=\frac{8(9)}{2}=36.</me> And use <m>t_8</m> to find another example:

<me>t_{4(8)(8+1)}=t_{288}=\frac{288\cdot289}{2}=41616=204^2.</me>
    </p>
    
</subsection>
-->

<subsection xml:id="Question_2_1_7">
    <title> Problem 7</title>
    <p>
        <md>
            <mrow>t_n^2-t_{n-1}^2\amp=\frac{n^2(n+1)^2}{4}-\frac{(n-1)^2(n)^2}{4}</mrow>
            <mrow>\amp=\frac{n^2(4n)}{4}</mrow>
            <mrow>\amp=n^3</mrow>
        </md>
    </p>
</subsection>

<!--

<subsection xml:id="Question_2_1_8">
    <title> Problem 8</title>
    <p>
        <md>
            <mrow>\frac{1}{1}+\frac{1}{3}+\dots+\frac{1}{t_n}\amp=\frac{2}{1(1+1)}+\frac{2}{2(2+1)}+\dots+\frac{2}{n(n+1)}</mrow>
            <mrow>\amp=2\cdot\left(\frac{1}{1}-\frac{1}{2}+\frac{1}{2}-\frac{1}{3}+\frac{1}{3}-\frac{1}{4}+\dots+\frac{1}{n}-\frac{1}{n-1}\right)</mrow>
            <mrow>\amp=2\cdot\left(1-\frac{1}{n+1}\right)&lt;2</mrow>
        </md>

since <m>1-\frac{1}{n+1}&lt;1</m>.
    </p>
    </subsection>
-->

    <subsection xml:id="Question_2_1_10">
    <title> Problem 10</title>
    <p>
        Use induction.  The key algebraic step is:

<md>
<mrow>\frac{(n-1)(3(n-1)-1)}{2}+(3n-2)\amp=\frac{(n-1)(3n-4)}{2}+(3n-2)</mrow>
<mrow>\amp=\frac{(n-1)(3n-4)+2(3n-2)}{2}</mrow>
<mrow>\amp=\frac{3n^2-n}{2}</mrow>
<mrow>\amp=\frac{n(3n-1)}{2}</mrow>
</md>
    </p>
</subsection>

 <subsection xml:id="Question_2_1_11">
    <title> Problem 11</title>
    <ol marker="(a)">
        <li>
            <!-- 
            <m>\phantom{empty}</m>
            <p>
                <me>
\frac{(n-1)(n)}{2}+n^2=\frac{3n^2-n}{2}=\frac{n(3n-1)}{2}</me>

            </p>-->
        </li>
        <li><m>\phantom{empty}</m>
            <p>
                <md>
                <mrow>3t_{n-1}+n\amp=3\frac{(n-1)(n)}{2}+n</mrow>
                <mrow>\amp=\frac{3n^2-3n+2n}{2}</mrow>
                <mrow>\amp=\frac{3n(n-1)}{2}=p_n</mrow>
                </md>
            


<md>
<mrow>2t_{n-1}+t_n\amp=2\frac{(n-1)(n)}{2}+\frac{n(n+1)}{2}</mrow>
<mrow>\amp=\frac{2n^2-2n+n^2+n}{2}</mrow>
<mrow>\amp=\frac{3n^2-n}{2}</mrow>
<mrow>\amp=\frac{3n(n-1)}{2}=p_n</mrow>
</md>
            </p>
        </li>
    </ol>
    
</subsection>






        </section>
    <!--/article-->
<!--/pretext-->