<?xml version="1.0" encoding="UTF-8"?>

<!--pretext-->
    <!--article xml:id="Sec_2_3"-->
        <section xml:id="Section_2_3">
        <title>Section 2.3</title>
        

<subsection xml:id="Question_2_3_2">
    <title> Problem 2</title>
    <ol marker="(a)">  
        <li>
            <p>
                If <m>a|b</m>, there exists <m>s</m> such that <m>as=b</m>. Then <m>asc=bc=a(sc)=bc</m> so <m>a|bc</m>.
            </p>
        </li>

        <li>
            <p>
                If <m>a|b</m> and <m>a|c</m> then there exist integers <m>s,t</m> such that <m>as=b</m> and <m>at=c</m>. Multiply these two equations: <m>a^2st=a^2(st)=bc</m>, so <m>a^2|bc</m>.
            </p>
        </li>

        <li>
            <p>
                If <m>a|b</m> then <m>as=b</m> for some integer <m>s</m>. Then <m>asc=ac(s)=bc</m> so <m>ac|bc</m>. Conversely, if <m>ac|bc</m> then <m>act=bc</m> for some integer <m>t</m>. Divide by <m>c</m> to obtain <m>at=b</m>, so <m>a|b</m>.
            </p>
        </li>

        <li>
            <p>
                similar
            </p>
        </li>
    </ol>
</subsection>        

<subsection xml:id="Question_2_3_3">
    <title> Problem 3</title>
    <p>
        This is false.  For example: <m>a=5, b=2, c=3</m>.
    </p>
</subsection>


<subsection xml:id="Question_2_3_5">
    <title> Problem 5</title>
    <p>
        By the division algorithm, <m>a=3q</m>, <m>a=3q+1</m>, or <m>a=3q+2</m>. 
        <ul>
            <li>
                <p>
                    If <m>a=3q</m>, then <m>3|a</m>.
                </p>
            </li>
            <li>
                <p>
                    If <m>a=3q+1</m>, then <m>a+2=3q+3=3(a+1)</m>, and <m>3|(a+2)</m>.
                </p>
            </li>
            <li>
                <p>
                    If <m>a=3q+2</m>, then <m>a+4=3q+6=3(q+2)</m>, and <m>3|(a+4)</m>.
                </p>
            </li>
        </ul>
    </p>
</subsection>

<subsection xml:id="Question_2_3_7">
    <title> Problem 7</title>
    <p>
        <md>
            <mrow>a^4+b^4-2 \amp (2k+1)^4+(2l+1)^4-2</mrow>
        </md>
        
    </p>

</subsection>

<subsection xml:id="Question_2_3_12">
    <title> Problem 12</title>
    <p> Let <m>d=\text{gcd}(a, a+n).</m> We'll use Theorem 2.2(g):
        <m>d|a</m> and <m>d|(a+n)</m> so <m>d|(a+n)-a</m>, that is <m>d|n</m>.  With <m>n=1</m> we have <m>\text{gcd}(a, a+1)|1</m> so it must be that <m>\text{gcd}(a,a+1)=1.</m>
    </p>
</subsection>
     
<subsection xml:id="Question_2_3_14">
    <title> Problem 14</title>
    <p>
        <ol marker="(a)">   
            <li> 
                We want to find integers <m>x</m> and <m>y</m> such that <me>x(2a+1)+y(9a+4)=1</me>.

        Rearrange to obtain: <me>a(2x+9y)+(x+4y)</me> and solve the system of equations:
        <md>
            <mrow>2x+9y \amp =0</mrow>
            <mrow>x+4y \amp = 1.</mrow>
        </md>

        A solution is <m>y=-2</m>, <m>x=9</m>: <me> 9(2a+1)-2(9a+4)=1</me>.  By Theorem 2.4 <me>\text{gcd}(2a+1, 9a+4)=1.</me>
        
        
            </li>
            <li>
                <p>
                    <me>-7(5a+2)+5(7a+3)=1</me>
                </p>
            </li>

            <li>
                <p>Let <m>d=\text{gcd}(3a, 3a+2)</m>.
                    Since <m>d|3a</m> and <m>d|3a+2</m>, then <m>d|(3a+2)-(3a)</m>. That is, <m>d|2</m>. So, either <m>d=1</m> or <m>d=2</m>.  But, <m>2 \nmid 3a</m> since <m>2 \nmid 3</m> and <m>2 \nmid a</m> (<m>a</m> is odd). So, <m>d=1</m>.
                </p>
            </li>
        </ol>
    </p>
</subsection>

<subsection xml:id="Question_2_3_15">
    <title> Problem 15</title>
    <p>
    Let <m>d=\text{gcd}(2a-3b, 4a-5b)</m>. Then <m>d|2a-3b</m> and <m>d|4a-5b</m>.  By Theorem 2.2(g) <m>d|-2(2a-3b)+(4a-5b)</m>.  That is, <m>d|b</m>. Let <m>b=-1</m> to obtain the result.
    </p>
</subsection>

<subsection xml:id="Question_2_3_20">
    <title> Problem 20</title>
    <ol marker="(a)">
        <li>
            <p>
                The hint is basically the solution.  
            </p>
        </li>

        <li>
            <p>
                There exist integers <m>x,y</m> such that <m>ax+by=1</m>. Since <m>c|a</m>, there exists an integer <m>k</m> such that <m>ck=a</m>. Then <m>c(kx)+by=1</m>, so <m>\text{gcd}(b,c)=1</m>.
            </p>
        </li>

        <li>
            <p>
                If <m>\text{gcd}(c,b)=1</m>, then <m>\text{gcd}(ac,b)=1</m> by part (a) and we are finished. 
            </p> 

               <p> Suppose <m>\text{gcd}(c,b)=d&gt; 1</m>. Since <m>d|c</m>, <m>d|ac</m>. Also <m>d|b</m>, so <m>d|\text{gcd}(ac,b)</m>.
               </p>
               <p>
                Let <m>\hat{d}=\text{gcd}(ac,b)</m>. Since <m>d &gt; 1</m> and since <m>d|\hat{d}</m>, <m>\hat{d}&gt;1</m>.  Now, <m>\hat{d}|ac</m> and <m>\hat{d}\nmid a</m>
                since <m>\text{gcd}(a,b)=1</m>. So, <m>\hat{d}|c</m> by Euclid's lemma. Hence <m>\hat{d}|\text{gcd}(c,b)</m>. That is <m>d|\hat{d}</m> and <m>\hat{d}|d</m>, so <m>d=\hat{d}</m>.</p>
            
        </li>

        <li>
            <p>
                see hint
            </p>
        </li>

        <li>
            <p>
                There exist integers <m>x,y</m> such that <m>xa+yb=1</m>.  Multiply by <m>c</m> to obtain <m>xac+ybc=c</m>.  Now if <m>d|ac</m> and <m>d|bc</m>, then <m>d|xac+ybc</m> by Theorem 2.2(g).  This gives <m>d|c</m> since <m>xac+ybc=c</m>.
            </p>
        </li>


    </ol>
</subsection>

        </section>
    <!--/article-->
<!--/pretext-->