<?xml version="1.0" encoding="UTF-8"?>

<!--pretext-->
    <!--article xml:id="Sec_1_2"-->
        <section xml:id="Section_1_2">
        <title>Section 1.2</title>
        
            
<subsection xml:id="Problem_1_2_1">
<title> Problem 1</title>
<p>


<md>
<mrow>\binom{n}{k} \binom{k}{r}\amp=\frac{n!}{k!(n-k)!}\cdot \frac{k!}{r!(k-r)!}</mrow>
<mrow> \amp=\frac{n!}{r!}\cdot \frac{1}{(n-k)!}\cdot \frac{1}{(k-r)!}</mrow>
<mrow> \amp= \frac{n!}{r!(n-r)!}\cdot \frac{1}{(n-k)!}\cdot \frac{(n-r)!}{(k-r)!}</mrow>
<mrow> \amp= \frac{n!}{r!(n-r)!}\cdot \frac{1}{((n-r)-(k-r))!}\cdot \frac{(n-r)!}{(k-r)!}</mrow>
<mrow> \amp=\binom{n}{r}\binom{n-r}{k-r}</mrow>
</md>

Let <m>r=1</m> in the identity:

<md>
<mrow>\binom{n}{k}\binom{k}{1}\amp=\binom{n}{1}\binom{n-1}{k-1}</mrow>
<mrow>\binom{n}{k}\amp=\frac{n}{k}\cdot \frac{(n-1)!}{(k-1)!((n-1)-(k-1))!}</mrow>
<mrow> \amp=\frac{n!}{k\cdot (k-1)!\cdot (n-k)!}</mrow>
<mrow> \amp=\frac{n-k+1}{k}\cdot \frac{n!}{(k-1)!(n-k)!(n-k+1)}</mrow>
<mrow> \amp= \frac{n-k+1}{k}\cdot \frac{n!}{(k-1)!((n-k+1)!)}</mrow>
<mrow> \amp= \frac{n-k+1}{k}\cdot\binom{n}{k-1}</mrow>
</md>

       
</p>
       
</subsection>



<subsection xml:id="Problem_1_2_3">
<title> Problem 3</title>
<p>


<ol marker="(a)">

<li> If <m>a=b=1</m> the binomial theorem is precisely the desired identity. </li>



<li> Similar idea: let <m>a=1</m> and <m>b=-1</m> in the binomial theorem. </li>



<li>
    
<me>(1+b)^{n}=\binom{n}{0}1^{n}+\binom{n}{1}(1)^{n-1}b+\binom{n}{2}b^2+\binom{n}{3}b^3+\cdots+\binom{n}{n}b^n</me>


Differentiating with respect to <m>b</m> gives:
<md><mrow>n(1+b)^{n-1}=\binom{n}{1}+2\binom{n}{2}b+3\binom{n}{3}b^2+\cdots+n\binom{n}{n}b^{n-1}</mrow></md>

Setting <m>b=1</m> gives the desired result.
</li>

<li><p>
    Use the expansion of <m>(1+b)^n</m> with <m>b=2</m>.
</p></li>

<li>Follow the hint.  Make sure to justify both equalities.
</li>

<li>
    <p> First:
        <md>
<mrow>(1-1)^{n+1}\amp=\binom{n+1}{0}+\binom{n+1}{1}(-1)^1+\binom{n+1}{2}+\cdots+\binom{n+1}{n+1}(-1)^{n+1}</mrow>
<mrow>\amp= \binom{n+1}{0}-\binom{n+1}{1}+\binom{n+1}{2}+\cdots+(-1)^{n+1}\binom{n+1}{n+1}</mrow>
        </md>

Each of the binomial terms is of the form
<me>\binom{n+1}{k}=\frac{(n+1)!}{k!(n+1-k)!}=\frac{n+1}{k}\cdot\frac{n!}{(k-1)!(n-k+1)!}=\frac{n+1}{k}\binom{n}{k-1}.</me>

Apply this to each term above on the right except the first:

<md>
<mrow>0\amp=1-\frac{n+1}{1}\binom{n}{0}+\frac{n+1}{2}\binom{n}{1}-\frac{n+1}{3}\binom{n}{2}+\cdots + (-1)^{n+1}\frac{n+1}{n+1}\binom{n}{n}</mrow>
<mrow>\frac{1}{n+1}\amp=\binom{n}{0}-\frac{1}{2}\binom{n}{1}+\frac{1}{3}\binom{n}{2}+\cdots+(-1)^n\frac{1}{n+1}\binom{n}{n}</mrow>
</md>
    </p>
</li>

</ol>

</p>
</subsection>

<subsection xml:id="Problem_1_2_4">
<title> Problem 4</title>
<p>



<me>\binom{n}{r}=\frac{n!}{r!(n-r)!}</me>
<me>\binom{n}{r+1}=\frac{n!}{(r+1)!(n-r-1)!}</me>


So <md>
<mrow>\binom{n}{r} &lt;\binom{n}{r+1}  \amp \phantom{4+5} \text{  iff  } \phantom{4+5} r!(n-r)!&gt;(r+1)!(n-r-1)!</mrow>
<mrow> \amp \phantom{4+5} \text{  iff  } \phantom{4+5} n-r  &gt;r+1</mrow>
<mrow> \amp \phantom{4+5} \text{  iff  } \phantom{4+5} n-1  &gt;2r</mrow>
<mrow> \amp \phantom{4+5} \text{  iff } \phantom{4+5} \frac{1}{2}(n-1)  &gt; r.</mrow>
</md>

Of course, we need <m>r \geq 0</m>.

The other parts are similar.

</p>
</subsection>

<!--

**6.**

$$\begin{align*}
\binom{2}{2}+\binom{4}{2}+ \cdots+\binom{2n}{2}&=\binom{2}{2}+2\binom{2}{2}+2^2+2\binom{3}{2}+3^2+\cdots +2\binom{n}{2}+n^2\\
&=\binom{2}{2}+2\left(\binom{2}{2}+\binom{3}{2}+\cdots \binom{n}{2}\right)+2^2+3^3+\cdots+n^2\\
&=2\binom{n+1}{3}+\frac{n(n+1)(2n+1)}{6}\\
&=2\frac{(n+1)!}{3!(n-2)!}+ \frac{n(n+1)(2n+1)}{6}\\
&=\frac{2(n+1)!+n(n+1)(2n+1)(n-2)!}{3!(n-2)!}\\
&=\frac{(n-2)!(2(n+1)(n)(n-1)+n(n+1)(2n+1))}{3!(n-2)!}\\
&=\frac{2(n+1)(n)(n-1)+n(n+1)(2n+1))}{6}\\
&=\frac{n(n+1)(2(n-1)+(2n+1))}{6}\\
&=\frac{n(n+1)(4n-1)}{6}
\end{align*}$$

Letâ€™s prove the hint:

$$\begin{align*}
\binom{2m}{2}&=\frac{(2m)!}{2!(2m-2)!}\\
&=\frac{(2m)(2m-1)}{2}\\
&=2m^2-m\\
&=m^2+m^2-m
\end{align*}$$

and since $$\begin{align*}
2\binom{m}{2}&=2\frac{m!}{2!(m-2)!}\\
&=m(m-1)\\
&=m^2-m
\end{align*}$$

we're done.

-->

<!--
**7.**

Use induction:

$$\begin{align*}
\binom{2n+1}{3}+(2n+1)^2&=\frac{(2n+1)!}{3!(2n-2)!}+(2n+1)^2\\
&=\frac{(2n+1)(2n)(2n-1)}{3!}+(2n+1)^2\\
&=\frac{(2n+1)(2n)(2n-1)+6(2n+1)^2}{3!}\\
&=\frac{(2n+1)((2n)(2n-1)+6(2n+1))}{3!}\\
&=\frac{(2n+1)(4n^2+10n+6)}{3!}\\
&=\frac{(2n+1)(2(2n^2+5n+3))}{3!}\\
&=\frac{2(2n+1)(2n+3)(n+1)}{3!}\\
&=\frac{(2n+3)(2n+2)(2n+1)(2n)!}{3!(2n)!}\\
&=\frac{(2n+3)!}{3!(2n+3-3)!}
\end{align*}$$

-->

<!--
**8.**

$$\begin{align*}
\binom{2n}{n} &= \frac{(2n)!}{n!n!}\\ \\
&=\frac{(2n)(2n-1)(2n-2)(2n-3)(2n-4)\cdots(5)(4)(3)(2)(1)}{[(n)(n-1)(n-2)\cdots(4)(3)(2)(1)][(n)(n-1)(n-2)\cdots(4)(3)(2)(1)]}\\ \\
&=\frac{2^n\cdot(n)(2n-1)(n-1)(2n-3)(n-2)\cdots(5)(2)(3)(1)(1)}{[(n)(n-1)(n-2)\cdots(4)(3)(2)(1)][(n)(n-1)(n-2)\cdots(4)(3)(2)(1)]}\\ \\
&= \frac{2^n\cdot(2n-1)(2n-3)\cdots(5)(3)(1)}{[(n)(n-1)(n-2)\cdots(4)(3)(2)(1)]}\\ \\
&= \frac{2^{2n}\cdot(2n-1)(2n-3)\cdots(5)(3)(1)}{2^n[(n)(n-1)(n-2)\cdots(4)(3)(2)(1)]}\\ \\
&= \frac{2^{2n}\cdot(2n-1)(2n-3)\cdots(5)(3)(1)}{(2n)(2n-2)(2n-4)\cdots(8)(6)(4)(2)}\\ \\
\end{align*}$$

**9.**

Using #8, this is equivalent to:

$$\frac{1}{2^n}< \frac{1\cdot3\cdot5\cdots(2n-1)}{2\cdot4\cdot6 \cdots (2n)} < 1.$$

Consider the fraction as:

$$\left(\frac{1}{2}\right)\left(\frac{3}{4}\right)\left(\frac{5}{6}\right)\cdots\left(\frac{2n-1}{2n}\right).$$

Each of these fractions is less than one, so the product is less than one, which gives the righthand inequality.

With the exception of $\frac{1}{2}$, each of these fractions is greater than $\frac{1}{2}$.  There are $n$ factors so the product is greater than $\frac{1}{2^n}$.


-->

        </section>
    <!--/article-->
<!--/pretext-->