<?xml version="1.0" encoding="UTF-8"?>

<!--pretext-->
    <!--article xml:id="Sec_1_1"-->
        <section xml:id="Section_1_1">
        <title>Section 1.1</title>
        
            
<subsection xml:id="Problem_1_1_6">
<title> Problem 6</title>
<!--
<exercise number="6">


<statement>
</statement>    
<answer>-->
<p>


For <m>n=4</m>: <m>4!=24</m> and <m>4^2=16</m> so the inequality holds.  Assume <m>n!>n^2</m> and consider:


<md>
<mrow>(n+1)!\amp =(n+1)\cdot n!</mrow>
<mrow>\amp &gt; (n+1)\cdot n^2  \text{ by the inductive hypothesis } </mrow>
<mrow>\amp &gt; (n+1)\cdot (n+1)</mrow>
<mrow>\amp =(n+1)^2.</mrow>
</md>


The second inequality requires that we prove <m>n^2>n+1</m> for <m>n\geq 4</m>. The following inequalities are equivalent:
<md>
<mrow>n^2 \amp &gt; n+1</mrow>
<mrow>n^2-n-1 \amp &gt;0</mrow>
<mrow>(n-2)(n+1)\amp &gt;0.</mrow>
</md>

The last inequality is true if <m>n&lt;-1</m> or <m>n&gt;2</m>.  So, <m>n^2&gt;n+1</m> for <m>n\geq 4 </m>.

We have shown that <m>n!&gt;n^2</m> implies <m>(n+1)!&gt;(n+1)^2</m>, and we have shown the inequality is true for <m>n=4</m>.  By induction, <m>n!&gt;n^2</m> is true for all integers <m>n\geq 4</m>.
       
       
</p>
<!-- </answer>       
</exercise>-->
</subsection>

<!--

<subsection xml:id="Problem_1_1_7">
<title> Problem 7</title>

<p>
    (quiz or exam)
For <m>n=1</m>: <md>1(1!)=2!-1</md>

Consider:

<md>
    <mrow> 1(1!)+2(2!)+\dots+n(n!)+(n+1)((n+1)!)\amp=(n+1)!-1+(n+1)(n+1)!  </mrow>
    <mrow> \amp =(n+1)!(1+n+1)-1</mrow>
    <mrow> \amp=(n+1)!(n+2)-1 </mrow>
    <mrow> \amp=(n+2)!-1 </mrow>
</md>
</p>

</subsection>

-->

<subsection xml:id="Problem_1_1_8">
<title> Problem 8</title>

<p>
For <m>n=1</m>: <md>2=\frac{2!}{1!}.</md>

Assume the identity is true for <m>n</m> and consider:

<md>
<mrow>2\cdot 6 \cdot 10 \cdots (4n-2)\cdot (4n+2)\amp=\frac{(2n)!}{n!}\cdot (4n+2)</mrow>
<mrow> \amp=\frac{(2n)!\cdot 2 \cdot (2n+1)}{n!}</mrow>
<mrow> \amp = \frac{(2n)!\cdot 2 \cdot (2n+1)\cdot (n+1)}{n!\cdot (n+1)}</mrow>
<mrow> \amp= \frac{(2n)! \cdot (2n+1)\cdot (2n+2)}{n!\cdot (n+1)}</mrow>
<mrow> \amp=\frac{(2(n+1))!}{(n+1)!}=\frac{(2n+2)!}{(n+1)!}</mrow>
</md>
which shows the identity is true for <m>n+1</m>. By induction the identity is true for all integers <m>n\geq1</m>.

The inequality <md><mrow>2^n(n!)^2\leq(2n)!</mrow></md>
is equivalent to <md><mrow>2^n(n!) \leq \frac{(2n)!}{n!}</mrow></md> so from part (a), we need to show that <md><mrow>2^n(n!) \leq 2\cdot 6 \cdot 10 \cdots (4n-2).</mrow></md>

The right hand side is:
<md>
<mrow>2\cdot 6 \cdot 10 \cdots (4n-2)\amp=(2\cdot1)\cdot(2\cdot3)\cdot(2\cdot 5)\cdots (2\cdot (2n-1))</mrow>
<mrow> \amp=2^n\cdot (1\cdot 3 \cdot 5 \cdots (2n-1))</mrow>
</md>



Clearly <md><mrow>n! \leq (1 \cdot 3 \cdot 5 \cdot (2n-1))</mrow> </md> since there are <m>n</m> factors in both products and all but the first factor are greater in the right hand side.  For example, if <m>n=4</m>: <md><mrow>1\cdot 2 \cdot 3 \cdot 4 \leq 1 \cdot 3 \cdot 5 \cdot 7.</mrow></md>  
Multiply both sides of <md><mrow>n! \leq (1 \cdot 3 \cdot 5 \cdot (2n-1))</mrow></md> by <m>2^n</m> to obtain the desired result.
</p>
</subsection>

<subsection xml:id="Problem_1_1_9">
<title> Problem 9</title>

<p>


For <m>n=1</m>, <m>1+a \geq 1+a</m>.

Assume <m>(1+a)^n \geq 1+na</m>  and consider <m>(1+a)^{n+1}</m>:

<md>>
<mrow>(1+a)^{n+1}\amp=(1+a)^n(1+a)</mrow>
<mrow> \amp \geq (1+na)(1+a)</mrow>
<mrow> \amp =1+na+a+na^2</mrow>
<mrow> \amp =1+(n+1)a+na^2</mrow>
<mrow>\geq 1+(n+1)a</mrow>
</md>

The first inequality follows from the inductive hypothesis. 
This first inequality is also where we need to use the assumption that <m>1+a &lt; 0</m>.  If <m>1+a&lt; 0</m>, the direction of the inequality would change. 
The second inequality is true since <m>na^2\geq 0</m>.


</p>
</subsection>


<subsection xml:id="Problem_1_1_10">
<title> Problem 10</title>

<p>


(a)

The following is not a complete proof or explanation.  It is only the algebra part. 
Make sure you can identify where the induction hypothesis is used.  Make sure you can justify both of the inequalities.

<md>
<mrow>\frac{1}{1^2}+\frac{1}{2^2}+\dots+\frac{1}{n^2}+\frac{1}{(n+1)^2}\amp\leq 2-\frac{1}{n}+\frac{1}{(n+1)^2}</mrow>
<mrow> \amp =2-\left(\frac{1}{n}-\frac{1}{(n+1)^2}\right)</mrow>
<mrow> \amp=2-\left(\frac{(n+1)^2-n}{n(n+1)^2}\right)</mrow>
<mrow> \amp=2-\left(\frac{n^2+n+1}{n(n+1)^2}\right)</mrow>
<mrow> \amp=2-\left(\frac{n^2+n+1}{(n^2+n)(n+1)}\right)</mrow>
<mrow> \amp\leq 2-\left(\frac{n^2+n+1}{(n^2+n+1)(n+1)}\right)</mrow>
<mrow> \amp=2-\frac{1}{n+1}</mrow>
</md>

(b)
 Again, the following is only the algebra.  It does not constitute a complete proof.

<md>
<mrow>2-\frac{n+2}{2^n}+\frac{n+1}{2^{n+1}}\amp=2-\left(\frac{n+2}{2^n}-\frac{n+1}{2^{n+1}}\right)</mrow>
<mrow> \amp=2-\frac{(2n+4)-(n+1)}{2^{n+1}}</mrow>
<mrow> \amp= 2-\frac{n+3}{2^{n+1}}</mrow>
</md>

</p>
</subsection>

<!--

<subsection xml:id="Problem_1_1_9_11">
<title> Problem 11</title>

<p>
 (save for exam)




<md>
<mrow>\frac{(2n+2)!}{2^{n+1}(n+1)!}\amp=\frac{(2n)!(2n+1)(2n+2)}{2^n\cdot2\cdot n!\cdot (n+1)}</mrow>
<mrow> \amp=\left(\frac{(2n)!}{2^nn!}\right)\left(\frac{(2n+1)(2n+2)}{2(n+1)}\right)</mrow>
<mrow> \amp= \left(\frac{(2n)!}{2^nn!}\right)(2n+1)</mrow>
</md>

So, if <md><mrow>\frac{(2n)!}{2^nn!}</mrow></md> is an integer, then so is <md><mrow>\frac{(2n+2)!}{2^{n+1}(n+1)!}.</mrow></md>

If <m>n=1</m> the expression equals <m>1</m>, an integer.

</p>
</subsection>

-->


        </section>
    <!--/article-->
<!--/pretext-->