<?xml version="1.0" encoding="UTF-8"?>

<!--pretext-->
    <!--article xml:id="Sec_2_3"-->
        <section xml:id="Section_2_4">
        <title>Section 2.4</title>
        

<subsection xml:id="Question_2_4_2">
    <title> Problem 2</title>
    <ol marker="(a)">
        <li><m>\phantom{blank line}</m>
            <p>
                <md>
                    <mrow>72 \amp =56\cdot 1 +16</mrow>
                    <mrow>56 \amp =16\cdot 3+8</mrow>
                    <mrow> 16  \amp = 8 \cdot 2 +0 </mrow>
                </md>
                So, <m>\text{gcd}(72, 56)=8</m>
                Working backwards:
                <md>
                    <mrow>8 \amp = 56-16\cdot 3</mrow>
                    <mrow> \amp =56-(72- 56)\cdot 3</mrow>
                    <mrow> \amp = 4\cdot 56-3\cdot 72</mrow>
                </md>

                which is the desired linear combination of <m>56</m> and <m>72</m>.
            
                
            </p>
        </li>
    </ol>
    The other parts follow the same process.

</subsection>        

     <subsection xml:id="Question_2_4_4">
    <title> Problem 4</title>
    <ol marker="(a)">
        <li>
            <!--
            <p>
                See the hint.
            </p>
        -->
        </li>

        <li>
            <!--
            <p>
                
            </p>
        -->
        </li>

        <li>
            <p>
                From the hint we have
                <md>
                    \text{gcd}(a+b, a^2+b^2)=\text{gcd}(a+b, (a+b)(a-b)+2b^2)
                </md>

                Let <m>d=\text{gcd}(a+b, a^2+b^2)</m>. Then <m>d|a+b</m>, and <m>d|(a+b)(a-b)+2b^2</m>. Since <m>d|a+b</m>, <m>d|(a+b)(a-b)</m>. It follows that <m>d|2b^2</m>
            </p>
               
            
            <p>
                We claim <m>\text{gcd}(d,b)=1</m>.  
            Suppose not, and there is a prime <m>p</m> that divides <m>d</m> and <m>b</m>.  Then <m>p|a+b</m> which implies that <m>p|a</m>. But that contradicts the assumption that <m>\text{gcd}(a,b)=1.</m>  
            </p>
           
           <p>
            If <m>\text{gcd}(d,b)=1</m>, then so too <m>\text{gcd}(d, b^2)=1</m>. Euclid's Lemmas then gives that <m>d|2</m> since <m>d|2b^2</m> and <m>\text{gcd}(d, b^2)=1.</m> If <m>d|2</m> then <m>d=1</m> or <m>d=2</m>.
                
                
            </p>
        </li>

        <li>
            <!--
            <p>
                
                Using the hint we have 
                <md>
                    d|a+b
                </md>
                and 
                <md>
                    d|(a+b)^2-3ab
                </md>
                from which we can conclude that
                <md>
                    d|3ab.
                </md>

                Next, we claim <m>\text{gcd}(d,a)=1</m>. Suppose there is an integer <m>k. &gt; 1</m>such that <m>k|d</m> and <m>d|a</m>.  Then also <m>k|a+b</m> which implies that <m>k|b.</m> This contradicts the assumption that <m>\text{gcd}(a,b)=1.</m>. Similarly, <m>\text{gcd}(d,b)=1</m>.  Now, since <m>d|3ab</m> we have <m>d|3</m> by Euclid's lemma.  Thus, <m>d=1</m> or <m>d=3</m>.
                
                
                
            </p>
        -->
        </li>
    </ol>
     </subsection>

<!--
     <subsection xml:id="Question_2_4_5">
    <title> Problem 5</title>
    <ol marker="(a)">
            <li>
                <p>
                    This follows from repeated use of the result from problem 20(a) in Section 2.2.
                    If <m>\text{gcd}(a,b)=1</m> and <m>\text{gcd}(a,b)=1</m>, then <m>\text{gcd}(a,b^2)=1</m>.  Continue until you have <m>\text{gcd}(a,b^n)=1.</m> Now think of this as <m>\text{gcd}(b^n,a)=1</m> and <m>\text{gcd}(b^n,a)</m> and problem 20(a) gives <m>\text{gcd}(b^n,a^2)=1.</m> Continue until you have <m>\text{gcd}(a^n, b^n).</m>. (A more careful presentation of this proof is inductive, but this is the idea.  Watch out for a result from chapter 3 which will give a "nicer" proof of this result.)
                </p>
            </li>

            <li>
                <p>Let <m>\text{gcd}(a,b)=d</m>. By the Corollary to Theorem 2.4 <m>\text{gcd}(a/d, b/d)=1</m>. Let <m>r=a/d</m> and <m>s=b/d</m>. By part (a) of the problem <m>\text{gcd}(r^n,s^n)=1</m>
                    Since <m>a=rd</m> and <m>b=sd</m>, we have <m>a^n=r^nd^n</m> and <m>b^n=s^nd^n</m>
                </p>
                <p>
                    Now, <m>a=rd</m> and <m>b=sd</m>, so <m>a^n=r^nd^n</m> and <m>b^n=s^nd^n</m>. Apply the hypotheseis that <m>a^n|b^n</m> to rewrite the second equatio: <m>b^n=ka^n=s^nd^n</m>.  Substitute the expression for <m>a^n</m> to obtain <m>kr^nd^n=s^nd^n</m>. Or <m>kr^n=s^n</m>. Now, suppose <m>r \neq 1</m>. Then there is some prime <m>p</m> such that <m>p|r</m>. From  <m>kr^n=s^n</m> we see this implies that <m>p|s^n</m>.  But this contradicts the fact that <m>\text{gcd}(r^n, s^n)=1</m>.
                </p>
                <p>
                    Hence <m>r=1</m> which gives <m>a=d</m>. Since <m>d|b</m> this yields the desired result.
                </p>
            </li>
        </ol>
    </subsection>
    -->
    
    <subsection xml:id="Question_2_4_6">
    <title> Problem 6</title>
    <p>
        Suppose <m>\text{gcd}(a+b, ab) \neq 1</m>. Then there is some prime <m>p</m> such that <m>p|\text{gcd}(a+b, ab)</m>. We claim <m>p</m> must divide at least one of <m>a</m> or <m>b</m>.  Suppose <m>p \nmid a</m>, then <m>\text{gcd}(a,p)=1</m> and by Euclid's lemmas we'd have <m>p|b</m>.  Similarly if <m>p\nmid b</m> we'd have <m>p|a</m>. Suppose, without loss of generality, that <m>p|a</m>.  Since also, <m>p|a+b</m> we have <m>p|b</m>. This contradicts the assumption that <m>\text{gcd}(a,b)=1</m>.  Thus, it must be that <m>\text{gcd}(a+b, ab)=1.</m>
           
               
            
       
    </p>
    </subsection>
        </section>
    <!--/article-->
<!--/pretext-->